Bignum.Component: Split into submodules

Bignum/Component/Extra.lean
@@ -6,7 +6,7 @@ Author: Guilherme Lima
 module
 
 public import Bignum.BitVec
-public import Bignum.Component
+public import Bignum.Component.Basic
 
 @[expose] public section
 
@@ -14,10 +14,13 @@ set_option autoImplicit false
 
 namespace Bignum.Component
 
-/-- Component for a bit within a BitVec. -/
+/-- Component for a bit within a bitvector. -/
 def bitelement {w : Nat} (i : Fin w) : Component (BitVec w) Bool :=
   ⟨λ bv ↦ bv.getLsb i, λ b bv ↦ BitVec.setLsb bv i b⟩
 
-/- Component for subwords of a BitVec. -/
+/-- Component for subwords of a bitvector. -/
+def subword {w : Nat} (start len : Nat) :
+    Component (BitVec w) (BitVec len) :=
+  ⟨BitVec.extractLsb' start len, λ b bv ↦ bv.overwriteLsb' start len b⟩
 
 end Bignum.Component
