BignumTest/ComponentExtra.lean
@@ -4,16 +4,32 @@ Released under Apache 2.0 license as described in the file LICENSE.
 Author: Guilherme Lima
 -/
 
-import Bignum.ComponentExtra
+import Bignum.Component.Extra
 
 open Bignum
 
-section bitelement
+-- bitelement
+
+namespace bitelementNS
 def bv : BitVec 8 := 0b01001011#8
 example : (Component.bitelement 0).read bv = true := by rfl
 example : (Component.bitelement 1).read bv = true := by rfl
 example : (Component.bitelement 2).read bv = false := by rfl
 example : (Component.bitelement 3).read bv = true := by rfl
-def bv' := (Component.bitelement 3).write false bv
-example : bv' = 0b01000011#8 := by rfl
-end bitelement
+example : (Component.bitelement 3).write false bv = 0b01000011#8 := by rfl
+namespace bitelementNS
+
+-- subword
+
+namespace subwordNS
+def bv : BitVec 8 := 0b01001011#8
+example : (Component.subword 0 3).read bv == 0b11#3 := by rfl
+example : (Component.subword 4 1).read bv == 0#1 := by rfl
+example : (Component.subword 0 0).read bv == 0#0 := by rfl
+example : (Component.subword 6 3).read bv == 1#3 := by rfl
+example : (Component.subword 7 3).read bv == 0#3 := by rfl
+example : (Component.subword 100 2).read bv == 0#2 := by rfl
+example : (Component.subword 0 3).write 0 bv == 0b01001000#8 := by rfl
+example : (Component.subword 1 3).write 0b101 bv == 0b01001011#8 := by rfl
+example : (Component.subword 6 4).write 0xf bv == 0b11001011#8 := by rfl
+end subwordNS
